added lookup function (this repo should now work with the main branch of the dy* repo)

dy-extensions/DY.Extend.fst
@@ -1,5 +1,399 @@
 module DY.Extend
 
+open Comparse
 open DY.Core
 open DY.Lib
+open DY.Core.Trace.Base
 
+val event_exists_grows:
+  #label_t:Type -> 
+  tr1:trace_ label_t -> tr2:trace_ label_t -> 
+  e:trace_event_ label_t ->
+  Lemma
+  (requires
+    tr1 <$ tr2 /\ event_exists tr1 e
+  )
+  (ensures
+    event_exists tr2 e
+  )
+let event_exists_grows tr1 tr2 e =  ()
+
+val last_entry_exists:
+  #label_t:Type ->
+  tr:trace_ label_t ->
+  Lemma
+    (requires Snoc? tr )
+    (ensures (
+       let Snoc _ last = tr in
+       event_exists tr last
+    ))
+    [SMTPat (Snoc? tr)]
+let last_entry_exists tr = 
+  let Snoc _ last = tr in
+  assert(event_at tr (length tr - 1) last)
+
+
+val get_state_aux_state_was_set:
+  prin:principal -> sess_id:state_id -> tr:trace ->
+  Lemma
+  (ensures (
+    match get_state_aux prin sess_id tr with
+    | None -> True
+    | Some content -> 
+          state_was_set tr prin sess_id content
+  ))
+let rec get_state_aux_state_was_set prin sess_id tr =
+   match tr with
+  | Nil -> ()
+  | Snoc tr_init (SetState prin' sess_id' content) -> (
+    if prin = prin' && sess_id = sess_id' 
+    then ()
+    else get_state_aux_state_was_set prin sess_id tr_init
+  )
+  | Snoc tr_init _ ->
+         get_state_aux_state_was_set prin sess_id tr_init
+
+val get_state_state_was_set:
+  prin:principal -> sess_id:state_id -> tr:trace ->
+  Lemma
+  (ensures (
+    let (opt_content, tr_out) = DY.Core.get_state prin sess_id tr in
+    tr == tr_out /\ (
+      match opt_content with
+      | None -> True
+      | Some content -> 
+             state_was_set tr prin sess_id content
+    )
+  ))
+  [SMTPat (DY.Core.get_state prin sess_id tr)]
+let get_state_state_was_set prin sess_id tr =
+  reveal_opaque (`%DY.Core.get_state) DY.Core.get_state;
+  get_state_aux_state_was_set prin sess_id tr
+  
+
+
+/// Lookup the most recent state of a principal satisfying some property.
+/// Returns the state and corresponding state id,
+/// or `None` if no such state exists.
+
+val lookup_state_aux: principal -> (bytes -> bool) -> trace -> option (bytes & state_id)
+let rec lookup_state_aux prin p tr =
+  match tr with
+  | Nil -> None
+  | Snoc rest (SetState prin' sid' cont') ->
+      if prin' = prin && p cont'
+      then Some (cont', sid')
+      else lookup_state_aux prin p rest
+  | Snoc rest _ -> lookup_state_aux prin p rest
+
+val core_lookup_state: principal -> (bytes -> bool) -> traceful (option (bytes & state_id))
+let core_lookup_state prin p =
+  let* tr = get_trace in
+  return (lookup_state_aux prin p tr)
+
+/// If `lookup` returns some state,
+/// this state satisfies the property used in the lookup.
+
+val lookup_state_aux_state_was_set_and_prop:
+  prin:principal -> p:(bytes -> bool) -> tr:trace ->
+  Lemma
+  (ensures (
+    let opt_content = lookup_state_aux prin p tr in
+      match opt_content with
+      | None -> True
+      | Some (content, sid) ->
+               p content
+             /\ state_was_set tr prin sid content
+  ))
+let rec lookup_state_aux_state_was_set_and_prop prin p tr =
+  match tr with
+  | Nil -> ()
+  | Snoc tr_init _ ->
+         lookup_state_aux_state_was_set_and_prop prin p tr_init
+
+/// If `lookup` returns a state on a trace with `trace_invariant`,
+/// the returned state additionally satisfies the state predicate.
+
+val lookup_state_aux_state_invariant:
+  {|protocol_invariants|} ->
+  prin:principal -> p:(bytes -> bool) -> tr:trace ->
+  Lemma
+  (requires
+    trace_invariant tr
+  )
+  (ensures (
+    let opt_content = lookup_state_aux prin p tr in
+      match opt_content with
+      | None -> True
+      | Some (content, sid) ->
+               state_pred.pred tr prin sid content
+             /\ p content
+             /\ state_was_set tr prin sid content
+  ))
+let lookup_state_aux_state_invariant #invs prin p tr =
+  lookup_state_aux_state_was_set_and_prop prin p tr;
+  match lookup_state_aux prin p tr with
+  | None -> ()
+  | Some (content, sid) ->
+    DY.Core.state_was_set_implies_pred tr prin sid content
+
+/// lifting both properties from `_aux` to the `traceful` versions.
+
+val core_lookup_state_state_was_set_and_prop:
+  prin:principal -> p:(bytes -> bool) -> tr:trace ->
+  Lemma
+  (ensures (
+    let (opt_content, tr_out) = core_lookup_state prin p tr in
+    tr == tr_out /\
+    (match opt_content with
+     | None -> True
+     | Some (content, sid) ->
+              p content
+            /\ state_was_set tr prin sid content
+    )
+  ))
+  [SMTPat (core_lookup_state prin p tr)]
+let core_lookup_state_state_was_set_and_prop prin p tr =
+  lookup_state_aux_state_was_set_and_prop prin p tr
+
+
+val lookup_state_state_invariant:
+  {|invs:protocol_invariants|} ->
+  prin:principal -> p:(bytes -> bool) -> tr:trace ->
+  Lemma
+  (requires
+    trace_invariant tr
+  )
+  (ensures (
+    let (opt_content, tr_out) = core_lookup_state prin p tr in
+    tr == tr_out /\
+    (match opt_content with
+     | None -> True
+     | Some (content, sid) ->
+              state_pred.pred tr prin sid content
+            /\ p content
+            /\ state_was_set tr prin sid content
+    )
+  ))
+  [SMTPat (core_lookup_state prin p tr); SMTPat (trace_invariant #invs tr)]
+let lookup_state_state_invariant #invs prin p tr =
+  lookup_state_aux_state_invariant prin p tr
+
+
+// val tagged_state_was_set_grows:
+//   tr1:trace -> tr2:trace ->
+//   tag:string -> p:principal -> sid:state_id -> cont:bytes ->
+//   Lemma
+//   (requires
+//      tr1 <$ tr2 /\ tagged_state_was_set tr1 tag p sid cont
+//   )
+//   (ensures
+//     tagged_state_was_set tr2 tag p sid cont
+//   )
+// let tagged_state_was_set_grows tr1 tr2 tag p sid cont = 
+//   reveal_opaque (`%tagged_state_was_set) tagged_state_was_set
+
+
+/// Lookup the most recent tagged state for a principal that satisfys some property.
+/// The property given as argument is on the _content_ of the state.
+
+val lookup_tagged_state:
+ string -> principal -> (bytes -> bool) -> traceful (option (bytes & state_id))
+let lookup_tagged_state the_tag prin p =
+  let p_ b =
+    match parse tagged_state b with
+    | None -> false
+    | Some ({tag; content;}) -> tag = the_tag && p content in
+  let*? (full_content_bytes, sid) = core_lookup_state prin p_ in
+  match parse tagged_state full_content_bytes with
+    | None -> return None
+    | Some ({tag; content;}) ->
+        if (tag = the_tag)
+        then return (Some (content, sid))
+        else return None
+
+
+val get_tagged_state_state_was_set:
+  tag:string -> 
+  prin:principal -> sess_id:state_id -> tr:trace ->
+  Lemma
+  (ensures (
+    let (opt_content, tr_out) = get_tagged_state tag prin sess_id tr in
+    tr == tr_out /\ (
+      match opt_content with
+      | None -> True
+      | Some content -> (
+         tagged_state_was_set tr tag prin sess_id content
+      )
+    )
+  )
+  )
+  [SMTPat (get_tagged_state tag prin sess_id tr)]
+let get_tagged_state_state_was_set tag prin sess_id tr =
+  reveal_opaque (`%get_tagged_state) (get_tagged_state);
+  reveal_opaque (`%tagged_state_was_set) (tagged_state_was_set);
+  let (opt_content, tr_out) = get_tagged_state tag prin sess_id tr in
+  match opt_content with
+  | None -> ()
+  | Some cont -> (
+    let (Some full_cont_bytes, _) = DY.Core.get_state prin sess_id tr in
+    serialize_parse_inv_lemma #bytes tagged_state full_cont_bytes    
+  )
+
+val lookup_tagged_state_pred:
+  tag:string ->
+  prin:principal -> p:(bytes -> bool) -> tr:trace ->
+  Lemma
+  (ensures (
+    let (opt_content, tr_out) = lookup_tagged_state tag prin p tr in
+    tr == tr_out /\
+    (match opt_content with
+     | None -> True
+     | Some (content,sid) ->
+           p content
+         /\ tagged_state_was_set tr tag prin sid content
+    )
+  ))
+  [SMTPat (lookup_tagged_state tag prin p tr);
+  ]
+let lookup_tagged_state_pred the_tag prin p tr =
+  let (opt_content, tr_out) = lookup_tagged_state the_tag prin p tr in
+  match opt_content with
+  | None -> ()
+  | Some (cont, sid) -> (
+  reveal_opaque (`%tagged_state_was_set) (tagged_state_was_set);
+  let p_ b =
+    match parse tagged_state b with
+    | None -> false
+    | Some ({tag; content;}) -> tag = the_tag && p content in
+  let (Some (full_cont_bytes, sid), _) = core_lookup_state prin p_ tr in
+  serialize_parse_inv_lemma #bytes tagged_state full_cont_bytes
+  )
+
+val lookup_tagged_state_invariant:
+  {|protocol_invariants|} ->
+  tag:string -> spred:local_bytes_state_predicate ->
+  prin:principal -> p:(bytes -> bool) -> tr:trace ->
+  Lemma
+  (requires
+    trace_invariant tr /\
+    has_local_bytes_state_predicate (tag, spred)
+  )
+  (ensures (
+    let (opt_content, tr_out) = lookup_tagged_state tag prin p tr in
+    tr == tr_out /\
+    (match opt_content with
+     | None -> True
+     | Some (content,sid) ->
+           spred.pred tr prin sid content
+         /\ p content
+         /\ tagged_state_was_set tr tag prin sid content
+    )
+  ))
+  [SMTPat (lookup_tagged_state tag prin p tr);
+   SMTPat (trace_invariant tr);
+   SMTPat (has_local_bytes_state_predicate (tag, spred))]
+let lookup_tagged_state_invariant #invs the_tag spred prin p tr =
+  reveal_opaque (`%has_local_bytes_state_predicate) (has_local_bytes_state_predicate);
+  let (opt_content, tr_out) = lookup_tagged_state the_tag prin p tr in
+  match opt_content with
+  | None -> ()
+  | Some (content,sid) -> (
+      let p_ b =
+        match parse tagged_state b with
+        | None -> false
+        | Some ({tag; content;}) -> tag = the_tag && p content in
+
+      let (Some (l_cont, l_sid), _) = core_lookup_state prin p_ tr in
+      serialize_parse_inv_lemma #bytes tagged_state l_cont;
+      reveal_opaque (`%tagged_state_was_set) (tagged_state_was_set);
+
+      let (Some (full_content_bytes, sid), tr) = core_lookup_state prin p_ tr in
+      local_eq_global_lemma split_local_bytes_state_predicate_params state_pred.pred the_tag spred (tr, prin, sid, full_content_bytes) the_tag (tr, prin, sid, content)
+     )
+
+/// Lookup the most recent state of a principal that satisfys some property.
+
+val lookup_state:
+  #a:Type -> {|local_state a|} ->
+  principal -> (a -> bool) -> traceful (option (a & state_id))
+let lookup_state #a #ls prin p =
+  let p_ b =
+    match parse a b with
+    | None -> false
+    | Some x -> p x in
+  let*? (content_bytes, sid) = lookup_tagged_state ls.tag prin p_ in
+  match parse a content_bytes with
+  | None -> return None
+  | Some content -> return (Some (content,sid))
+
+
+val lookup_state_pred:
+  #a:Type -> {|ls:local_state a|} ->
+  prin:principal -> p:(a -> bool) -> tr:trace ->
+  Lemma
+  (ensures (
+    let (opt_content, tr_out) = lookup_state prin p tr in
+    tr == tr_out /\
+    (match opt_content with
+     | None -> True
+     | Some (content, sid) ->
+          p content
+          /\ DY.Lib.state_was_set tr prin sid content
+    )
+  ))
+  [SMTPat (lookup_state #a #ls prin p tr);
+   ]
+let lookup_state_pred #a #ls prin p tr =
+  let (opt_content, tr_out) = lookup_state prin p tr in
+  match opt_content with
+  | None -> ()
+  | Some (content, sid) -> (
+      let p_ b =
+        match parse a b with
+        | None -> false
+        | Some x -> p x in
+      let (Some (l_cont, l_sid), _) = lookup_tagged_state ls.tag prin p_ tr in
+     serialize_parse_inv_lemma #bytes a l_cont;
+     reveal_opaque (`%DY.Lib.state_was_set) (DY.Lib.state_was_set #a)
+  )
+
+
+
+val lookup_state_invariant:
+  #a:Type -> {|local_state a|} ->
+  {|protocol_invariants|} ->
+  spred:local_state_predicate a ->
+  prin:principal -> p:(a -> bool) -> tr:trace ->
+  Lemma
+  (requires
+    trace_invariant tr /\
+    has_local_state_predicate spred
+  )
+  (ensures (
+    let (opt_content, tr_out) = lookup_state prin p tr in
+    tr == tr_out /\
+    (match opt_content with
+     | None -> True
+     | Some (content, sid) ->
+         spred.pred tr prin sid content
+         /\ p content
+         /\ DY.Lib.state_was_set tr prin sid content
+    )
+  ))
+  [SMTPat (lookup_state #a prin p tr);
+   SMTPat (trace_invariant tr);
+   SMTPat (has_local_state_predicate spred)]
+let lookup_state_invariant #a #ls #invs spred prin p tr =
+  let (opt_content, tr_out) = lookup_state prin p tr in
+  match opt_content with
+  | None -> ()
+  | Some (content, sid) -> (
+      let p_ b =
+        match parse a b with
+        | None -> false
+        | Some x -> p x in
+      let (Some (l_cont, l_sid), _) = lookup_tagged_state ls.tag prin p_ tr in
+      serialize_parse_inv_lemma #bytes a l_cont;
+      reveal_opaque (`%DY.Lib.state_was_set) (DY.Lib.state_was_set #a)
+  )
